WIP: small progress on instrument

io/ILang.CompileTo.TLang.fst
@@ -14,49 +14,6 @@ open IO.Sig
 open DM.IIO
 open TC.Checkable
 
-assume val dynamic_cmd :
-  (cmd : io_cmds) ->
-  (d1 : checkable2 (io_pre cmd)) ->
-  (arg : io_sig.args cmd) ->
-  IIOwp (io_resm cmd)
-    (fun p h ->
-      (forall (r:(io_sig.res cmd arg)) lt.
-        (match r with
-         | Inr Contract_failure -> ~(d1.check2 arg h) /\ lt == []
-         | _ -> d1.check2 arg h /\ lt == [convert_call_to_event cmd arg r]) ==> p lt r))
-
-let run_m
-  (pi:monitorable_prop)
-  (tree : iio 'b) :
-  IIOpi 'b pi =
-  admit ();
-  let tree : dm_iio 'b (fun p h -> forall (r: 'b) (lt: trace). enforced_locally pi h lt ==> p lt r) = tree in
-  IIOwp?.reflect tree
-
-let rec _instrument
-  (tree : iio (resexn 'a))
-  ('p    : monitorable_prop)
-  (piprop:squash (forall h cmd arg. 'p cmd arg h ==> io_pre cmd arg h)) :
-  IIOpi (resexn 'a) 'p =
-  match tree with
-  | Return r -> r
-  | Call GetTrace argz fnc -> Inr Contract_failure
-  | PartialCall pre fnc -> Inr Contract_failure
-  | Decorated d #b m k ->
-      let r : b = FStar.Universe.downgrade_val (run_m 'p m) in
-      admit ();
-      _instrument (k r) 'p piprop
-  | Call cmd argz fnc -> begin
-    let d : checkable2 (io_pre cmd) = (
-      implies_is_checkable2 (io_sig.args cmd) trace ('p cmd) (io_pre cmd) piprop) in
-    (** Check if the runtime check failed, and if yes, return the error **)
-    let rez = dynamic_cmd cmd d argz in
-    let z' : iio (resexn 'a) = fnc rez in
-    _instrument z' 'p piprop
-  end
-
-
-
 class compilable (t:Type) (pi:monitorable_prop) = {
   c_t_ilang : ilang t pi;
   comp_type : Type;
@@ -65,6 +22,16 @@ class compilable (t:Type) (pi:monitorable_prop) = {
   // CC theorem?
   // c_compile: squash (forall (wS:t). theta (reify (compile wS)) `hist_ord` theta (reify wS)) 
 }
+
+class instrumentable (t:Type) (pi:monitorable_prop) = {
+  cc_t_ilang : ilang t pi;
+  inst_type : Type;
+  c_inst_type : tlang inst_type;
+  c_pi:squash (forall h cmd arg. pi cmd arg h ==> io_pre cmd arg h);
+  instrument: inst_type -> t 
+}
+
+(** *** Compilable base types **)
 
 instance compile_resexn pi (t:Type) {| d1:compilable t pi |} : compilable (resexn t) pi = {
   c_t_ilang = ilang_resexn pi t #d1.c_t_ilang;
@@ -76,16 +43,10 @@ instance compile_resexn pi (t:Type) {| d1:compilable t pi |} : compilable (resex
     | Inr err -> Inr err)
 }
 
-class instrumentable (t:Type) (pi:monitorable_prop) = {
-  cc_t_ilang : ilang t pi;
-  inst_type : Type;
-  c_inst_type : tlang inst_type;
-  instrument: inst_type -> t 
-}
+(** *** Compilable arrows **)
 
-#push-options "--print_universes"
 (** TODO: t1 and t2 are in universe 0. is that a problem? can we do HO? **)
-instance compile_ilang_base (t1:Type u#0) (t2:Type u#0) pi {| d1:instrumentable t1 pi |} {| d2:compilable t2 pi |} : compilable (t1 -> IIOpi (resexn t2) pi) pi  = {
+instance compile_ilang_base (t1:Type u#0) (t2:Type u#0) pi {| d1:instrumentable t1 pi |} {| d2:compilable t2 pi |} : compilable (t1 -> IIOpi (resexn t2) pi) pi = {
   c_t_ilang = ilang_arrow pi t1 #d1.cc_t_ilang t2 #d2.c_t_ilang;
   comp_type = d1.inst_type -> MIIO (resexn d2.comp_type);
   c_comp_type = tlang_arrow d1.inst_type d2.comp_type #d1.c_inst_type #d2.c_comp_type;
@@ -100,4 +61,74 @@ instance compile_ilang_base (t1:Type u#0) (t2:Type u#0) pi {| d1:instrumentable 
     let dm : dm_iio (resexn d2.comp_type) (trivial_hist ()) = Decorated (fun h lt -> b2t (enforced_locally pi h lt)) x' Return in
     IIOwp?.reflect dm
   );
+}
+
+(** *** Insturmentable types **)
+instance instrumentable_resexn pi (t:Type) {| d1:instrumentable t pi |} : instrumentable (resexn t) pi = {
+  cc_t_ilang = ilang_resexn pi t #d1.cc_t_ilang;
+  inst_type = resexn (d1.inst_type);
+  c_inst_type = tlang_resexn d1.inst_type #d1.c_inst_type;
+  c_pi = d1.c_pi;
+  instrument = (fun x ->
+    match x with
+    | Inl r -> Inl (instrument r)
+    | Inr err -> Inr err)
+}
+
+
+(** *** Instrumentable arrows **)
+assume val dynamic_cmd :
+  (cmd : io_cmds) ->
+  (d1 : checkable2 (io_pre cmd)) ->
+  (arg : io_sig.args cmd) ->
+  IIOwp (io_resm cmd)
+    (fun p h ->
+      (forall (r:(io_sig.res cmd arg)) lt.
+        (match r with
+         | Inr Contract_failure -> ~(d1.check2 arg h) /\ lt == []
+         | _ -> d1.check2 arg h /\ lt == [convert_call_to_event cmd arg r]) ==> p lt r))
+
+let run_m
+  (pi:monitorable_prop)
+  (tree : dm_iio 'b (fun p h -> forall lt r. enforced_locally pi h lt ==> p lt r)) :
+  IIOpi 'b pi =
+  let tree : dm_iio 'b (fun p h -> forall (r: 'b) (lt: trace). enforced_locally pi h lt ==> p lt r) = tree in
+  IIOwp?.reflect tree
+
+let rec _instrument
+  (tree : dm_iio (resexn 'a) (trivial_hist ()))
+  (pi    : monitorable_prop)
+  (c_pi:squash (forall h cmd arg. pi cmd arg h ==> io_pre cmd arg h)) :
+  IIOpi (resexn 'a) pi =
+  match tree with
+  | Return r -> r
+  | Call GetTrace argz fnc -> Inr Contract_failure
+  | PartialCall pre fnc -> Inr Contract_failure
+  | Decorated d #b m k ->
+      assume (forall h. dm_iio_theta m (fun lt r -> enforced_locally pi h lt) h);
+      let r : b = FStar.Universe.downgrade_val (run_m pi m) in
+      let z' : iio (resexn 'a) = k r in
+      assume (trivial_hist () `hist_ord` dm_iio_theta z');
+      admit ();
+      _instrument z' pi c_pi
+  | Call cmd argz fnc -> begin
+    let d : checkable2 (io_pre cmd) = (
+      implies_is_checkable2 (io_sig.args cmd) trace (pi cmd) (io_pre cmd) c_pi) in
+    (** Check if the runtime check failed, and if yes, return the error **)
+    let rez = dynamic_cmd cmd d argz in
+    let z' : iio (resexn 'a) = fnc rez in
+    assume (trivial_hist () `hist_ord` dm_iio_theta z');
+    _instrument z' pi c_pi
+  end
+
+instance instrumentable_arrow t1 t2 pi {| d1:compilable t1 pi |} {| d2:instrumentable t2 pi |} : instrumentable (t1 -> IIOpi (resexn t2) pi) pi = {
+  cc_t_ilang = ilang_arrow pi t1 #d1.c_t_ilang t2 #d2.cc_t_ilang;
+  inst_type = d1.comp_type -> MIIO (resexn d2.inst_type);
+  c_inst_type = tlang_arrow d1.comp_type d2.inst_type #d1.c_comp_type #d2.c_inst_type;
+  c_pi = d2.c_pi;
+  instrument = (fun (f:d1.comp_type -> MIIO (resexn d2.inst_type)) (x:t1) -> 
+    let tree : dm_iio (resexn d2.inst_type) (trivial_hist ()) = reify (f (compile x)) in
+    let r  : resexn d2.inst_type = _instrument #d2.inst_type tree pi d2.c_pi in 
+    instrument #_ #pi #(instrumentable_resexn pi t2 #d2) r 
+  )
 }
